Autosubst4Lean/Test7/Syntax/Ty.lean
@@ -1,49 +1,45 @@
-import Autosubst4Lean.Test4.Debruijn
+import Autosubst4Lean.Test7.Debruijn
 
-namespace RegionCalc
+namespace RefCalc
 
 inductive Ty : Sig -> Type where
-| tvar : BVar s .tvar -> Ty s
-| arrow : Ty s -> Ty s -> Ty s
-| ref : BVar s .rvar -> Ty s -> Ty s
-| forallTy : Ty (s,X) -> Ty s
-| forallRgn : Ty (s,r) -> Ty s
 | unit : Ty s
+| arrow : Ty s -> Ty s -> Ty s
+| prod : Ty s -> Ty s -> Ty s
+| ref : BVar s .lvar -> Ty s -> Ty s
+| forallL : Ty (s,l) -> Ty s
 
 def Ty.rename : Ty s1 -> Rename s1 s2 -> Ty s2
-| .tvar x0, f => .tvar (f.var x0)
-| .arrow a0 a1, f => .arrow (a0.rename f) (a1.rename f)
-| .ref x0 a1, f => .ref (f.var x0) (a1.rename f)
-| .forallTy a0, f => .forallTy (a0.rename f.lift)
-| .forallRgn a0, f => .forallRgn (a0.rename f.lift)
 | .unit, _ => .unit
+| .arrow a0 a1, f => .arrow (a0.rename f) (a1.rename f)
+| .prod a0 a1, f => .prod (a0.rename f) (a1.rename f)
+| .ref x0 a1, f => .ref (f.var x0) (a1.rename f)
+| .forallL a0, f => .forallL (a0.rename f.lift)
 
 theorem Ty.rename_id {t : Ty s} :
     t.rename (Rename.id) = t := by
   induction t
-  case tvar => rfl
+  case unit => rfl
   case arrow =>
+    simp_all [Ty.rename]
+  case prod =>
     simp_all [Ty.rename]
   case ref =>
     simp_all [Ty.rename, Rename.id]
-  case forallTy =>
+  case forallL =>
     simp_all [Ty.rename, Rename.lift_id]
-  case forallRgn =>
-    simp_all [Ty.rename, Rename.lift_id]
-  case unit => rfl
 
 theorem Ty.rename_comp {t : Ty s1} {f : Rename s1 s2} {g : Rename s2 s3} :
     (t.rename f).rename g = t.rename (f.comp g) := by
   induction t generalizing s2 s3
-  case tvar => rfl
+  case unit => rfl
   case arrow =>
+    simp_all [Ty.rename]
+  case prod =>
     simp_all [Ty.rename]
   case ref =>
     simp_all [Ty.rename, Rename.comp]
-  case forallTy =>
+  case forallL =>
     simp_all [Ty.rename, Rename.lift_comp]
-  case forallRgn =>
-    simp_all [Ty.rename, Rename.lift_comp]
-  case unit => rfl
 
-end RegionCalc
+end RefCalc
