Autosubst4Lean/Test7/Syntax.lean
@@ -1,4 +1,2 @@
-import Autosubst4Lean.Test7.Syntax.CTy
-import Autosubst4Lean.Test7.Syntax.VTy
-import Autosubst4Lean.Test7.Syntax.Comp
-import Autosubst4Lean.Test7.Syntax.Val
+import Autosubst4Lean.Test7.Syntax.Ty
+import Autosubst4Lean.Test7.Syntax.Exp
