Autosubst4Lean/Test7/Syntax/Comp.lean
@@ -36,7 +36,7 @@ theorem Comp.rename_id {t : Comp s} :
   case app =>
     simp_all [Comp.rename, Val.rename_id]
   case lapp =>
-    simp_all [Comp.rename, Val.rename_id]
+    simp_all [Comp.rename, Val.rename_id, Rename.id]
   case fst =>
     simp_all [Comp.rename, Val.rename_id]
   case snd =>
@@ -44,11 +44,11 @@ theorem Comp.rename_id {t : Comp s} :
   case newrgn =>
     simp_all [Comp.rename, Rename.lift_id]
   case read =>
-    simp_all [Comp.rename, Val.rename_id]
+    simp_all [Comp.rename, Val.rename_id, Rename.id]
   case write =>
-    simp_all [Comp.rename, Val.rename_id]
+    simp_all [Comp.rename, Val.rename_id, Rename.id]
   case alloc =>
-    simp_all [Comp.rename, Val.rename_id]
+    simp_all [Comp.rename, Val.rename_id, Rename.id]
 
 theorem Comp.rename_comp {t : Comp s1} {f : Rename s1 s2} {g : Rename s2 s3} :
     (t.rename f).rename g = t.rename (f.comp g) := by
@@ -60,7 +60,7 @@ theorem Comp.rename_comp {t : Comp s1} {f : Rename s1 s2} {g : Rename s2 s3} :
   case app =>
     simp_all [Comp.rename, Val.rename_comp]
   case lapp =>
-    simp_all [Comp.rename, Val.rename_comp]
+    simp_all [Comp.rename, Val.rename_comp, Rename.comp]
   case fst =>
     simp_all [Comp.rename, Val.rename_comp]
   case snd =>
@@ -68,10 +68,10 @@ theorem Comp.rename_comp {t : Comp s1} {f : Rename s1 s2} {g : Rename s2 s3} :
   case newrgn =>
     simp_all [Comp.rename, Rename.lift_comp]
   case read =>
-    simp_all [Comp.rename, Val.rename_comp]
+    simp_all [Comp.rename, Val.rename_comp, Rename.comp]
   case write =>
-    simp_all [Comp.rename, Val.rename_comp]
+    simp_all [Comp.rename, Val.rename_comp, Rename.comp]
   case alloc =>
-    simp_all [Comp.rename, Val.rename_comp]
+    simp_all [Comp.rename, Val.rename_comp, Rename.comp]
 
 end RefCalc
