Autosubst4Lean/Test7/Syntax/Exp.lean
@@ -1,0 +1,104 @@
+import Autosubst4Lean.Test7.Debruijn
+import Autosubst4Lean.Test7.Syntax.Ty
+
+namespace RefCalc
+
+inductive Exp : Sig -> Type where
+| var : BVar s .var -> Exp s
+| unit : Exp s
+| pair : Exp s -> Exp s -> Exp s
+| abs : Ty s -> Exp (s,x) -> Exp s
+| labs : Exp (s,l) -> Exp s
+| ret : Exp s -> Exp s
+| bind : Exp s -> Exp (s,x) -> Exp s
+| app : Exp s -> Exp s -> Exp s
+| lapp : Exp s -> BVar s .lvar -> Exp s
+| fst : Exp s -> Exp s
+| snd : Exp s -> Exp s
+| newrgn : Exp (s,l) -> Exp s
+| read : BVar s .lvar -> Exp s -> Exp s
+| write : BVar s .lvar -> Exp s -> Exp s -> Exp s
+| alloc : BVar s .lvar -> Exp s -> Exp s
+
+def Exp.rename : Exp s1 -> Rename s1 s2 -> Exp s2
+| .var x0, f => .var (f.var x0)
+| .unit, _ => .unit
+| .pair a0 a1, f => .pair (a0.rename f) (a1.rename f)
+| .abs a0 a1, f => .abs (a0.rename f) (a1.rename f.lift)
+| .labs a0, f => .labs (a0.rename f.lift)
+| .ret a0, f => .ret (a0.rename f)
+| .bind a0 a1, f => .bind (a0.rename f) (a1.rename f.lift)
+| .app a0 a1, f => .app (a0.rename f) (a1.rename f)
+| .lapp a0 x1, f => .lapp (a0.rename f) (f.var x1)
+| .fst a0, f => .fst (a0.rename f)
+| .snd a0, f => .snd (a0.rename f)
+| .newrgn a0, f => .newrgn (a0.rename f.lift)
+| .read x0 a1, f => .read (f.var x0) (a1.rename f)
+| .write x0 a1 a2, f => .write (f.var x0) (a1.rename f) (a2.rename f)
+| .alloc x0 a1, f => .alloc (f.var x0) (a1.rename f)
+
+theorem Exp.rename_id {t : Exp s} :
+    t.rename (Rename.id) = t := by
+  induction t
+  case var => rfl
+  case unit => rfl
+  case pair =>
+    simp_all [Exp.rename]
+  case abs =>
+    simp_all [Exp.rename, Ty.rename_id, Rename.lift_id]
+  case labs =>
+    simp_all [Exp.rename, Rename.lift_id]
+  case ret =>
+    simp_all [Exp.rename]
+  case bind =>
+    simp_all [Exp.rename, Rename.lift_id]
+  case app =>
+    simp_all [Exp.rename]
+  case lapp =>
+    simp_all [Exp.rename, Rename.id]
+  case fst =>
+    simp_all [Exp.rename]
+  case snd =>
+    simp_all [Exp.rename]
+  case newrgn =>
+    simp_all [Exp.rename, Rename.lift_id]
+  case read =>
+    simp_all [Exp.rename, Rename.id]
+  case write =>
+    simp_all [Exp.rename, Rename.id]
+  case alloc =>
+    simp_all [Exp.rename, Rename.id]
+
+theorem Exp.rename_comp {t : Exp s1} {f : Rename s1 s2} {g : Rename s2 s3} :
+    (t.rename f).rename g = t.rename (f.comp g) := by
+  induction t generalizing s2 s3
+  case var => rfl
+  case unit => rfl
+  case pair =>
+    simp_all [Exp.rename]
+  case abs =>
+    simp_all [Exp.rename, Ty.rename_comp, Rename.lift_comp]
+  case labs =>
+    simp_all [Exp.rename, Rename.lift_comp]
+  case ret =>
+    simp_all [Exp.rename]
+  case bind =>
+    simp_all [Exp.rename, Rename.lift_comp]
+  case app =>
+    simp_all [Exp.rename]
+  case lapp =>
+    simp_all [Exp.rename, Rename.comp]
+  case fst =>
+    simp_all [Exp.rename]
+  case snd =>
+    simp_all [Exp.rename]
+  case newrgn =>
+    simp_all [Exp.rename, Rename.lift_comp]
+  case read =>
+    simp_all [Exp.rename, Rename.comp]
+  case write =>
+    simp_all [Exp.rename, Rename.comp]
+  case alloc =>
+    simp_all [Exp.rename, Rename.comp]
+
+end RefCalc
